src/Nontermination.v
@@ -49,6 +49,34 @@ Proof.
   intros n H; induction n; auto.
 Admitted.
 
+Definition div {Var : Set} : Code Var := V * (C * I * TOP).
+
+Lemma ap_top_div (Var : Set) (x : Code Var) : div * (x * TOP) == div * x.
+Proof.
+Admitted.
+
+Lemma div_ap_top (Var : Set) (x : Code Var) : div * x * TOP == div * x.
+Proof.
+  (* OLD
+  split.
+    rewrite beta_div at 2; rewrite pi_j_right; auto.
+  unfold code_le, conv; intros Var' c f H.
+  simpl in *; auto.
+  *)
+Admitted.
+
+Lemma div_repeat_top (Var : Set) (x : Code Var) (n : nat) :
+  (div * x) ** TOP ^^ n == div * x.
+Proof.
+  induction n; simpl; auto.
+Admitted.
+
+Lemma repeat_top_div (Var : Set) (x : Code Var) (n : nat) :
+  div * (x ** TOP ^^ n) == div * x.
+Proof.
+  induction n; simpl; auto.
+Admitted.
+
 Lemma div_probe_bot (Var : Set) :
   forall n : nat, ~ conv (probe n (@code_bot Var)).
 Proof.
