src/BohmTrees.v
@@ -4,6 +4,7 @@ Require Import Coq.Program.Basics.
 Require Import Coq.Setoids.Setoid.
 Require Import Coq.Classes.RelationClasses.
 Require Import Coq.Classes.Morphisms.
+Require Import Coq.Lists.List.
 Require Export InformationOrdering.
 Require Import Nontermination.
 Open Scope code_scope.
