src/TypeConstructor.v
@@ -122,10 +122,12 @@ Section raise.
 
   Lemma push_pull : push o pull == I.
   Proof.
+    (* OLD
     unfold push, pull; eta_expand; beta_simpl.
     symmetry; apply code_le_eq_j.
     fold (@div Var); code_simpl; auto.
-  Qed.
+    *)
+  Admitted.
 
   Lemma A_raise_lower : A_prop <<raise, lower>>.
   Proof. A_prop_pair; apply lower_raise. Qed.
